src/ConcurrentLog.v
@@ -14,8 +14,8 @@ Definition LogLength : var Mcontents nat := HFirst.
 (* we will store the log length in commit_sector *)
 Definition commit_sector : addr := $10.
 
-Inductive log_entry :=
-| LogEntry (a:addr) (v:valu).
+Record log_entry := { log_addr : addr;
+                      log_valu : valu }.
 
 Definition addr_record_type : Rec.type :=
   Rec.RecF [("addr", Rec.WordF addrlen);
@@ -28,13 +28,53 @@ Definition read_addr (v:valu) : addr :=
   Eval compute_rec in
     @Rec.of_word addr_record_type v :-> "addr".
 
-Definition log_write {T} a v rx : prog Mcontents S T :=
+Definition log_append {T} a v rx : prog Mcontents S T :=
   l <- Get LogLength;
   let off := (l+1)*2 in
   Write ($ off) (serialize_addr a);;
   Write ($ (off + 1)) v;;
   rx tt.
 
-Definition log_commit {T} rx : prog Mcontents S T :=
+Definition read_entry {T} n rx : prog Mcontents S T :=
+  av <- Read ($ (n * 2));
+  v <- Read ($ (n * 2 + 1));
+  rx (Build_log_entry (read_addr av) v).
+
+Definition write_entry {T} e rx : prog Mcontents S T :=
+  Write (log_addr e) (log_valu e);; rx tt.
+
+Definition log_write {T} rx : prog Mcontents S T :=
   l <- Get LogLength;
-  (* need a For loop... *)
+  _ <- For i < l
+| Ghost [ (_:unit) ]
+| Loopvar [ (_:unit) ]
+| Continuation lrx
+| LoopInv (fun d m s0 s => True)
+| OnCrash (fun d => True)
+| Begin
+    e <- read_entry i;
+  write_entry e;;
+              lrx (tt, tt)
+
+| Rof (tt, tt);
+  rx tt.
+
+Definition log_sync {T} rx : prog Mcontents S T :=
+  l <- Get LogLength;
+  _ <- For i < l
+| Ghost [ (_:unit) ]
+| Loopvar [ (_:unit) ]
+| Continuation lrx
+| LoopInv (fun d m s0 s => True)
+| OnCrash (fun d => True)
+| Begin
+    e <- read_entry i;
+  Sync (log_addr e);;
+       lrx (tt, tt)
+| Rof (tt, tt);
+  rx tt.
+
+Definition log_commit {T} rx : prog Mcontents S T :=
+  Write commit_sector $0;;
+        Sync commit_sector;;
+        rx tt.
